More refactoring.
MATTHIEU: I moved some stuff from L3 to Ast.Common, and made it
parametric on the language (L0 - L3).  In order to make L3_to_L4.v and
L3_to_L4_correct.v check I added a few long pathnames and parameter
arguments.

L5 MAINTAINER: I'm not sure why L5 refers to things in L3, but in
order to make some examples at the end of cpseval.v check, I changed
some type cast annotations.

theories/L3_flattenedApp/program.v
@@ -20,218 +20,6 @@ Local Open Scope list.
 Set Implicit Arguments.
 
 
-Inductive fresh (nm:string) : environ -> Prop :=
-| fcons: forall s p ec,
-         fresh nm p -> nm <> s -> fresh nm ((s,ec)::p)
-| fnil: fresh nm nil.
-Hint Constructors fresh.
-
-Lemma fresh_dec: forall nm p, (fresh nm p) \/ ~(fresh nm p).
-induction p.
-- left. auto.
-- destruct a. destruct IHp. destruct (string_dec nm s).
- + subst. right. intros h. inversion_Clear h. nreflexivity H4.
- + left. constructor; auto.
- + right. intros h. elim H. inversion_Clear h. assumption.
-Qed.
-
-Lemma fresh_tl: forall nm p, fresh nm p -> fresh nm (tl p).
-induction 1.
-- simpl. assumption.
-- auto.
-Qed.
-
-Lemma fresh_strengthen:
-  forall rs qs nm, fresh nm (rs++qs) -> fresh nm qs.
-induction rs; intros qs nm h.
-- assumption.
-- inversion h. subst. auto.
-Qed.
-
-Lemma fresh_not_head:
-  forall nm t p nmtp, fresh nm nmtp -> nmtp = ((nm,t)::p) -> False.
-induction 1; intros h.
-- inversion h. subst. auto.
-- discriminate h.
-Qed.
-
-
-(*** Common functions for evaluation ***)
-
-(** Lookup an entry in the environment **)
-Inductive Lookup: string -> environ -> envClass -> Prop :=
-| LHit: forall s p t, Lookup s ((s,t)::p) t
-| LMiss: forall s1 s2 p t ec,
-           s2 <> s1 -> Lookup s2 p ec -> Lookup s2 ((s1,t)::p) ec.
-Hint Constructors Lookup.
-
-Definition LookupDfn s p t := Lookup s p (ecTrm t).
-Definition LookupTyp s p n i := Lookup s p (ecTyp n i).
-
-(** equivalent functions **)
-Function lookup (nm:string) (p:environ) : option envClass :=
-  match p with
-   | nil => None
-   | cons (s,ec) p => if (string_eq_bool nm s) then Some ec
-                                 else lookup nm p
-  end.
-
-Function lookupDfn (nm:string) (p:environ) : option Term :=
-  match lookup nm p with
-   | Some (ecTrm t) => Some t
-   | _ => None
-  end.
-
-Lemma Lookup_lookup:
-  forall nm p t, Lookup nm p t -> lookup nm p = Some t.
-induction 1; intros; subst.
-- simpl. rewrite (string_eq_bool_rfl s). reflexivity.
-- simpl. rewrite (string_eq_bool_neq H). destruct t; assumption.
-Qed.
-
-Lemma lookup_Lookup:
-  forall nm p t, lookup nm p = Some t -> Lookup nm p t.
-induction p; intros t h. inversion h.
-destruct a. destruct (string_dec nm s); simpl in h.
-- subst. rewrite (string_eq_bool_rfl s) in h. 
-  injection h. intros; subst. apply LHit.
-- apply LMiss. assumption. apply IHp. 
-  rewrite (string_eq_bool_neq n) in h. assumption.
-Qed.
-
-Lemma not_lookup_not_Lookup:
- forall (nm:string) (p:environ) (ec:envClass),
-   ~(lookup nm p = Some ec) <-> ~(Lookup nm p ec).
-split; eapply deMorgan_impl.
-- apply (Lookup_lookup).
-- apply (lookup_Lookup).
-Qed.
-
-Lemma LookupDfn_lookupDfn:
-  forall nm p t, Lookup nm p t ->
-                 forall te, t = (ecTrm te) -> lookupDfn nm p = Some te.
-induction 1; intros; subst.
-- unfold lookupDfn, lookup. rewrite (string_eq_bool_rfl s). reflexivity.
-- unfold lookupDfn, lookup. rewrite (string_eq_bool_neq H).
-  destruct t; apply IHLookup; reflexivity.
-Qed.
-
-Lemma lookupDfn_LookupDfn:
-  forall nm p t, lookupDfn nm p = Some t -> Lookup nm p (ecTrm t).
-intros nm p t. 
-functional induction (lookupDfn nm p); intros h; try discriminate.
-- injection h. intros. subst. apply lookup_Lookup. assumption.
-Qed.
-
-
-(**
-Lemma LookupDfn_functional:
-  forall (nm:string) (p:environ) (t r:Term),
-    LookupDfn nm p t -> LookupDfn nm p r -> t = r.
-intros nm p t r h1 h2. 
-assert (j1:= LookupDfn_lookupDfn h1 (te:=t)).
-assert (j2:= LookupDfn_lookupDfn h2 (te:=r)).
-rewrite j1 in j2. injection j2; intros; subst; reflexivity. reflexivity.
-Qed.
-***)
-
-(***
-Lemma not_lookupDfn_not_LookupDfn:
- forall (nm:string) (p:environ) (t:Term),
-   ~(lookupDfn nm p = Some t) <-> ~(LookupDfn nm p t).
-split; eapply deMorgan_impl.
-- apply (proj2 (lookupDfn_LookupDfn _ _ _ )).
-- apply (proj1 (lookupDfn_LookupDfn _ _ _ )).
-Qed.
-
-Lemma lookupDfn_None_not_LookupDfn:
-  forall (nm:string) (p:environ) (t:Term),
-    lookupDfn nm p = None -> ~(LookupDfn nm p t).
-intros nm p te h. apply (proj1 (not_lookupDfn_not_LookupDfn _ _ _)). 
-intuition. rewrite h in H. discriminate.
-Qed.
-
-Lemma lookupDfn_neq:
-  forall n1 n2 p t, n1 <> n2 ->
-     lookupDfn n1 ((n2, ecConstr t) :: p) = lookupDfn n1 p.
-intros n1 n2 p t h.
-unfold lookupDfn. rewrite (string_eq_bool_neq h). reflexivity.
-Qed.
-
-Lemma LookupDfn_neq:
-  forall n1 n2 p t u, n1 <> n2 ->
-     LookupDfn n1 ((n2, ecConstr t) :: p) u -> LookupDfn n1 p u.
-intros n1 n2 p t u h1 h2.
-apply (proj1 (lookupDfn_LookupDfn _ _ _)).
-erewrite <- (lookupDfn_neq _ _ h1).
-apply (proj2 (lookupDfn_LookupDfn _ _ _)). eassumption.
-Qed.
-
-Lemma lookupDfn_eq:
-  forall n t p, lookupDfn n ((n, ecConstr t) :: p) = Some t.
-intros n t p.
-unfold lookupDfn. rewrite string_eq_bool_rfl. reflexivity.
-Qed.
-***)
-
-(***
-Lemma fresh_lookupDfn_fails:
-  forall s p, fresh s p <-> lookupDfn s p = None.
-split. 
-- induction 1.
-  + unfold lookupDfn. rewrite (string_eq_bool_neq H0).
-    apply IHfresh.
-  + reflexivity.
-- intros h. induction p.
-  + auto.
-  + destruct a. destruct e. destruct (string_dec s s0).
-    * rewrite e in h. simpl in h. rewrite string_eq_bool_rfl in h.
-      discriminate.
-    * eapply fcons. apply IHp. simpl in h. 
-      rewrite (string_eq_bool_neq n) in h. assumption. assumption.
-Qed.
-***)
-
-Lemma fresh_Lookup_fails:
-  forall nm p ec, fresh nm p -> ~(Lookup nm p ec).
-induction 1; intro h; inversion h; subst; auto.
-Qed.
-
-Lemma Lookup_strengthen:
-  forall (nm1:string) pp t, Lookup nm1 pp t -> 
-       forall nm2 ec p, pp = (nm2,ec)::p -> nm1 <> nm2 -> Lookup nm1 p t.
-intros nm1 pp t h nm2 ecx px j1 j2. subst. assert (k:= Lookup_lookup h).
-simpl in k. rewrite (string_eq_bool_neq j2) in k.
-apply lookup_Lookup. assumption.
-Qed.
-
-Lemma Lookup_fresh_neq:
-  forall nm2 p t, Lookup nm2 p t -> forall nm1, fresh nm1 p -> nm1 <> nm2.
-induction 1; intros.
-- inversion H. assumption.
-- apply IHLookup. apply (fresh_tl H1).
-Qed.
-
-Lemma Lookup_weaken:
-  forall s p t, Lookup s p t -> 
-      forall nm ec, fresh nm p -> Lookup s ((nm, ec) :: p) t.
-intros s p t h1 nm ec h2.
-assert (j1:= Lookup_fresh_neq h1 h2). apply LMiss. apply neq_sym. assumption.
-assumption.
-Qed.
-
-Lemma fresh_lookup_None: forall nm p, fresh nm p <-> lookup nm p = None.
-split. 
-- induction 1; simpl; try reflexivity.
-  + rewrite string_eq_bool_neq; assumption.
-- induction p; auto.
-  + destruct a. destruct (string_dec nm s). 
-    * subst. simpl. rewrite string_eq_bool_rfl. discriminate.
-    * simpl. rewrite string_eq_bool_neq; try assumption. intros h.
-      apply fcons; intuition.
-Qed.
-
-
 (** Check that a named datatype and constructor exist in the environment **)
 Definition defaultCnstr := {| CnstrNm:=""; CnstrArity:= 0 |}.
 Definition defaultItyp := {| itypNm:=""; itypCnstrs:=nil |}.
@@ -242,12 +30,12 @@ Definition CrctCnstr (ipkg:itypPack) (inum cnum:nat) : Prop :=
   else False.
 
 (** correctness specification for programs (including local closure) **)
-Inductive Crct: environ -> nat -> Term -> Prop :=
+Inductive Crct: (environ Term) -> nat -> Term -> Prop :=
 | CrctSrt: forall n s, Crct nil n (TSort s)
 | CrctWkTrmTrm: forall n p t s nm, Crct p n t -> Crct p n s ->
            fresh nm p -> Crct ((nm,ecTrm s)::p) n t
 | CrctWkTrmTyp: forall n p t s nm, Crct p n t -> CrctTyp p n s ->
-           fresh nm p -> forall m, Crct ((nm,ecTyp m s)::p) n t
+           fresh nm p -> forall m, Crct ((nm,ecTyp _ m s)::p) n t
 | CrctRel: forall n m p, m < n -> Crct p n prop -> Crct p n (TRel m)
 | CrctProd: forall n p nm bod,
             Crct p n prop -> Crct p (S n) bod -> Crct p n (TProd nm bod)
@@ -272,20 +60,20 @@ Inductive Crct: environ -> nat -> Term -> Prop :=
              Crct p n prop ->    (** convenient for IH *)
              CrctDs p (n + dlength ds) ds -> Crct p n (TFix ds m)
 | CrctInd: forall n p ind, Crct p n prop -> Crct p n (TInd ind)
-with Crcts: environ -> nat -> Terms -> Prop :=
+with Crcts: environ Term -> nat -> Terms -> Prop :=
 | CrctsNil: forall n p, Crct p n prop -> Crcts p n tnil
 | CrctsCons: forall n p t ts,
                Crct p n t -> Crcts p n ts -> Crcts p n (tcons t ts)
-with CrctDs: environ -> nat -> Defs -> Prop :=
+with CrctDs: environ Term -> nat -> Defs -> Prop :=
 | CrctDsNil: forall n p, Crct p n prop -> CrctDs p n dnil
 | CrctDsCons: forall n p dn db dra ds,
           Crct p n db -> CrctDs p n ds -> CrctDs p n (dcons dn db dra ds)
-with CrctTyp: environ -> nat -> itypPack -> Prop := 
+with CrctTyp: environ Term -> nat -> itypPack -> Prop := 
 | CrctTypStart: forall n itp, CrctTyp nil n itp
 | CrctTypWk1: forall n p t s nm, CrctTyp p n t -> Crct p n s ->
            fresh nm p -> CrctTyp ((nm,ecTrm s)::p) n t
 | CrctTypWk2: forall n p t s nm, CrctTyp p n t -> CrctTyp p n s ->
-           fresh nm p -> forall m, CrctTyp ((nm,ecTyp m s)::p) n t.
+           fresh nm p -> forall m, CrctTyp ((nm,ecTyp _ m s)::p) n t.
 Hint Constructors Crct Crcts CrctDs CrctTyp.
 Scheme Crct_ind' := Minimality for Crct Sort Prop
   with Crcts_ind' := Minimality for Crcts Sort Prop
@@ -299,17 +87,18 @@ Combined Scheme CrctCrctsCrctDs_ind from Crct_ind', Crcts_ind', CrctDs_ind'.
 Lemma Crct_WFTrm:
   (forall p n t, Crct p n t -> WFTrm t n) /\
   (forall p n ts, Crcts p n ts -> WFTrms ts n) /\
-  (forall (p:environ) (n:nat) (ds:Defs), CrctDs p n ds -> WFTrmDs ds n) /\
-  (forall (p:environ) (n:nat) (itp:itypPack), CrctTyp p n itp -> True).
+  (forall (p:environ Term) (n:nat) (ds:Defs), CrctDs p n ds -> WFTrmDs ds n) /\
+  (forall (p:environ Term) (n:nat) (itp:itypPack), CrctTyp p n itp -> True).
 apply CrctCrctsCrctDsTyp_ind; intros; try auto; try (solve [constructor]).
 Qed.
 
 Lemma Crct_up:
   (forall p n t, Crct p n t -> Crct p (S n) t) /\
   (forall p n ts, Crcts p n ts -> Crcts p (S n) ts) /\
-  (forall (p:environ) (n:nat) (ds:Defs), CrctDs p n ds -> CrctDs p (S n) ds) /\
-  (forall (p:environ) (n:nat) (itp:itypPack), CrctTyp p n itp ->
-                                              CrctTyp p (S n) itp).
+  (forall (p:environ Term) (n:nat) (ds:Defs),
+     CrctDs p n ds -> CrctDs p (S n) ds) /\
+  (forall (p:environ Term) (n:nat) (itp:itypPack),
+     CrctTyp p n itp -> CrctTyp p (S n) itp).
 apply CrctCrctsCrctDsTyp_ind; intros.
 - constructor.
 - apply CrctWkTrmTrm; assumption.
@@ -361,7 +150,7 @@ Qed.
 
 Lemma CrctTypTl:
   forall pp n t, Crct pp n t ->
-    forall nm npars tp p, pp = ((nm,ecTyp npars tp)::p) -> CrctTyp p n tp.
+    forall nm npars tp p, pp = ((nm,ecTyp _ npars tp)::p) -> CrctTyp p n tp.
 induction 1; intros; try discriminate;
 try (solve [eapply IHCrct2; eassumption]);
 try (solve [eapply IHCrct; eassumption]);
@@ -394,7 +183,7 @@ Lemma Crct_fresh_Pocc:
   (forall p n ts, Crcts p n ts -> forall nm, fresh nm p -> ~ PoccTrms nm ts) /\
   (forall p n (ds:Defs), CrctDs p n ds -> forall nm, fresh nm p ->
                                                      ~ PoccDefs nm ds) /\
-  (forall (p:environ) (n:nat) (itp:itypPack), CrctTyp p n itp -> True).
+  (forall (p:environ Term) (n:nat) (itp:itypPack), CrctTyp p n itp -> True).
 apply CrctCrctsCrctDsTyp_ind; intros; try intros j; auto;
 try (solve [inversion j]);
 try (solve [inversion_clear j; elim (H0 nm); trivial]);
@@ -402,7 +191,8 @@ try (solve [inversion_clear j; elim (H0 nm); trivial; elim (H2 nm); trivial]);
 try (solve [inversion_clear j; elim (H0 nm0); trivial; elim (H2 nm0); trivial]);
 try (solve [inversion_clear j; elim (H0 nm); trivial; elim (H2 nm); trivial]);
 try (solve [inversion_clear H4; elim (H0 nm0); trivial]).
-- inversion j. subst. elim (@fresh_Lookup_fails _ _ (ecTrm pd) H2). assumption.
+- inversion j. subst.
+  elim (@fresh_Lookup_fails _ _ _ (ecTrm pd) H2). assumption.
 - inversion_Clear j. 
   + eelim (fresh_Lookup_fails H5). eassumption.
   + eelim H4; eassumption.
@@ -415,7 +205,7 @@ Lemma Crct_not_bad_Lookup:
                  forall nm, LookupDfn nm p (TConst nm) -> False) /\
   (forall p n ds, CrctDs p n ds ->
                  forall nm, LookupDfn nm p (TConst nm) -> False) /\
-  (forall (p:environ) (n:nat) (itp:itypPack), CrctTyp p n itp -> True).
+  (forall (p:environ Term) (n:nat) (itp:itypPack), CrctTyp p n itp -> True).
 apply CrctCrctsCrctDsTyp_ind; intros; auto;
 try (solve [elim (H0 _ H3)]); try (solve [elim (H0 _ H5)]);
 try (solve [elim (H0 _ H1)]); try (solve [elim (H0 _ H2)]).
@@ -454,16 +244,16 @@ Qed.
 Lemma  Crct_Typ_weaken:
   (forall p n t, Crct p n t -> 
     forall nm itp, fresh nm p -> CrctTyp p n itp ->
-                   forall npars, Crct ((nm,ecTyp npars itp)::p) n t) /\
+                   forall npars, Crct ((nm,ecTyp _ npars itp)::p) n t) /\
   (forall p n ts, Crcts p n ts -> 
     forall nm itp, fresh nm p -> CrctTyp p n itp ->
-                 forall npars, Crcts ((nm,ecTyp npars itp)::p) n ts) /\
+                 forall npars, Crcts ((nm,ecTyp _ npars itp)::p) n ts) /\
   (forall p n ds, CrctDs p n ds -> 
     forall nm itp, fresh nm p -> CrctTyp p n itp ->
-                   forall npars, CrctDs ((nm,ecTyp npars itp)::p) n ds) /\
+                   forall npars, CrctDs ((nm,ecTyp _ npars itp)::p) n ds) /\
   (forall p n jtp, CrctTyp p n jtp -> 
     forall nm itp, fresh nm p -> CrctTyp p n itp ->
-                  forall npars,  CrctTyp ((nm,ecTyp npars itp)::p) n jtp).
+                  forall npars,  CrctTyp ((nm,ecTyp _ npars itp)::p) n jtp).
 Proof.
   eapply CrctCrctsCrctDsTyp_ind; intros; auto.
   - apply CrctWkTrmTyp; try assumption. eapply CrctConst; try eassumption.
@@ -480,7 +270,7 @@ Lemma Crct_strengthen:
                  ~ PoccTrms nm ss -> Crcts p n ss) /\
   (forall pp n ds, CrctDs pp n ds -> forall nm ec p, pp = (nm,ec)::p ->
                  ~ PoccDefs nm ds -> CrctDs p n ds) /\
-  (forall (pp:environ) (n:nat) (itp:itypPack), CrctTyp pp n itp -> True).
+  (forall (pp:environ Term) (n:nat) (itp:itypPack), CrctTyp pp n itp -> True).
 apply CrctCrctsCrctDsTyp_ind; intros; auto.
 - discriminate.
 - injection H4; intros. subst. assumption.
@@ -550,8 +340,9 @@ Proof.
 assert (lem: (forall p n t, Crct p n t -> 
                             forall nm u, LookupDfn nm p u -> Crct p n u) /\
              (forall p n ts, Crcts p n ts -> True) /\
-             (forall (p:environ) (n:nat) (ds:Defs), CrctDs p n ds -> True) /\
-             (forall (p:environ) (n:nat) (itp:itypPack),
+             (forall (p:environ Term) (n:nat) (ds:Defs),
+                CrctDs p n ds -> True) /\
+             (forall (p:environ Term) (n:nat) (itp:itypPack),
                 CrctTyp p n itp -> True)).
   { apply CrctCrctsCrctDsTyp_ind; intros; auto;
     try (solve [eapply H1; eassumption]);
@@ -579,7 +370,7 @@ Proof.
 Qed.
 
 Lemma Crct_invrt_WkTrm:
-  forall (ev:environ) n t, Crct ev n t ->
+  forall (ev:environ Term) n t, Crct ev n t ->
   forall nm s p, ev = (nm, ecTrm s)::p -> Crct p n s.
 Proof.
   induction 1; intros; try discriminate;
@@ -820,7 +611,7 @@ Qed.
 
 (*********
 (** An alternative correctness specification for programs: [crct], below **)
-Definition weaklyClosed (t:Term) (p:environ) : Prop :=
+Definition weaklyClosed (t:Term) (p:environ Term) : Prop :=
   forall nm, PoccTrm nm t -> lookupDfn nm p <> None.
 Fixpoint weaklyCloseds (ts:Terms) p : Prop :=
   match ts with
@@ -887,7 +678,7 @@ induction 1; intros nm h; unfold weaklyClosed.
     unfold weaklyClosed in IHLookupDfn. apply (IHLookupDfn _ h).
 Qed.
 
-Inductive envOk : environ -> Prop :=
+Inductive envOk : environ Term -> Prop :=
 | envOk_nil : envOk nil
 | envOk_cons : forall nm t p,
       fresh nm p -> envOk p -> weaklyClosed t p ->
@@ -965,8 +756,8 @@ apply CrctCrctsCrctDs_ind; intros; auto.
 Qed.
 
 
-Definition crct (p:environ) (t:Term) : Prop := envOk p /\ weaklyClosed t p.
-Fixpoint crcts (p:environ) (ts:Terms) : Prop :=
+Definition crct (p:environ Term) (t:Term) : Prop := envOk p /\ weaklyClosed t p.
+Fixpoint crcts (p:environ Term) (ts:Terms) : Prop :=
   match ts with
     | tnil => True
     | tcons s ss => crct p s /\ crcts p ss
